Fusion of contexts and Lcontexts

theories/Context.v
@@ -5,15 +5,80 @@ From LogRel Require Import Utils BasicAst.
 
 Set Primitive Projections.
 
+Definition LCon := list (prod nat bool).
+
+Inductive in_LCon : LCon -> nat -> bool -> Prop :=
+| in_here_l (l : LCon) {d b} : in_LCon (cons (d,b) l) d b
+| in_there_l {l : LCon} {d b d' b'} : in_LCon l d b -> in_LCon (cons (d',b') l) d b.
+
+Inductive not_in_LCon : LCon -> nat -> Prop :=
+| not_in_nil : forall n, not_in_LCon nil n
+| not_in_there : forall {l n m b}, n <> m -> not_in_LCon l n
+                                 -> not_in_LCon (cons (m,b) l) n.
+
+Inductive wf_LCon : LCon -> Prop :=
+| wf_nil : wf_LCon nil
+| wf_cons : forall {l n b}, wf_LCon l -> not_in_LCon l n -> wf_LCon (cons (n,b) l).
+
+Definition le_LCon l l' : Prop :=
+  forall n b, in_LCon l n b -> in_LCon l' n b.
+
+Definition le_LCon_refl l : le_LCon l l := fun n b ne => ne.
+
+Definition le_LCon_trans {l l' l''} :
+  le_LCon l l' -> le_LCon l' l'' -> le_LCon l l'' :=
+  fun le le' n b ne => le' n b (le n b ne).
+
+Fixpoint nSucc (n : nat) (t : term) : term :=
+  match n with
+  | 0 => t
+  | S n => tSucc (nSucc n t)
+  end.
+
+Definition nat_to_term (n : nat) : term := nSucc n tZero.
+
+Definition bool_to_term (b : bool) : term :=
+  match b with
+  | true => tTrue
+  | false => tFalse
+  end.
+
+Record SsigT (A : Type) (B : A -> Prop) :=
+  exist {pi1 : A ; pi2 : B pi1}.
+Arguments pi1 [_ _] _.
+Arguments pi2 [_ _] _.
+
+Definition wfLCon := SsigT LCon wf_LCon.
+
+Definition wfLCons (l : wfLCon) {n : nat} (ne : not_in_LCon (pi1 l) n) (b : bool) : wfLCon.
+Proof.
+  exists (cons (n,b) (pi1 l)).
+  econstructor ; trivial.
+  exact (pi2 l).
+Defined.
+
+
 (** ** Context declaration *)
 (** Context: list of declarations *)
 (** Terms use de Bruijn indices to refer to context entries.*)
 
-Definition context := list term.
+Definition context := prod (list term) (wfLCon).
 
-Notation "'ε'" := (@nil term).
-Notation " Γ ,, d " := (@cons term d Γ) (at level 20, d at next level).
-Notation " Γ ,,, Δ " := (@app term Δ Γ) (at level 25, Δ at next level, left associativity).
+Definition cons_con (Γ : context) (d : term) : context :=
+  ((@cons term d (fst Γ)) , snd Γ).
+
+Definition cons_lcon (Γ : context) {n : nat} (d : prod (not_in_LCon (pi1 (snd Γ)) n) bool) : context :=
+  (fst Γ , wfLCons (snd Γ) (fst d) (snd d)).
+
+Definition app_con (Γ : context) (l : list term) : context :=
+  (@app term l (fst Γ) , snd Γ).
+
+
+Notation "'ε' l" := ((@nil term) , l) (at level 20).
+Notation " Γ ,, d " := (@cons_con Γ d) (at level 20, d at next level).
+Notation " Γ ,,, Δ " := (app_con Γ (fst Δ)) (at level 25, Δ at next level, left associativity).
+Notation " Γ ',,l' d " := (cons_lcon Γ d) (at level 20, d at next level).
+
 
 (** States that a definition, correctly weakened, is in a context. *)
 Inductive in_ctx : context -> nat -> term -> Type :=
@@ -25,5 +90,56 @@ Lemma in_ctx_inj Γ n decl decl' :
 Proof.
   induction 1 in decl' |- * ; inversion 1 ; subst.
   1: reflexivity.
-  now f_equal.
+  f_equal.
+  apply IHin_ctx.
+  destruct Γ ; destruct Γ0.
+  cbn in * ; rewrite <- H3 ; now rewrite <- H4.
+Qed.
+
+
+Lemma notinLConnotinLCon {l n b} : not_in_LCon l n -> in_LCon l n b -> False.
+Proof.
+  intros notinl inl.
+  induction inl.
+  - inversion notinl ; subst.
+    now apply H3.
+  - eapply IHinl.
+    now inversion notinl ; subst.
+Qed.
+
+Lemma nattoterminj {n m} : nat_to_term n = nat_to_term m -> n = m.
+Proof.
+  revert m.
+  induction n ; cbn in *.
+  - induction m ; try reflexivity ; cbn.
+    intro H.
+    exfalso.
+    change (match tZero as t0 return Type with
+            | tZero => False
+            | _ => True
+            end).
+    now rewrite H.
+  - intros m H.
+    induction m ; cbn in *.
+    + exfalso.
+      change (match tZero as t0 return Type with
+              | tZero => False
+              | _ => True
+              end).
+      now rewrite <- H.
+    + erewrite (IHn m) ; try reflexivity.
+      now inversion H.
+Qed.
+
+Lemma uniqueinLCon {l n b b'} : wf_LCon l -> in_LCon l n b -> in_LCon l n b' -> b = b'.
+Proof.
+  intros wfl inl inl'.
+  induction wfl.
+  - now inversion inl.
+  - inversion inl ; subst.
+    + inversion inl' ; subst ; trivial.
+      exfalso ; exact (notinLConnotinLCon H H5).
+    + inversion inl' ; subst.
+      * exfalso ; exact (notinLConnotinLCon H H5).
+      * exact (IHwfl H5 H6).
 Qed.
